DeBruijnSSA/BinSyntax/Rewrite/Region/Compose/Elgot.lean
@@ -1,0 +1,75 @@
+import DeBruijnSSA.BinSyntax.Rewrite.Region.LSubst
+import DeBruijnSSA.BinSyntax.Rewrite.Region.Compose.Seq
+import DeBruijnSSA.BinSyntax.Rewrite.Region.Compose.Product
+import DeBruijnSSA.BinSyntax.Rewrite.Region.Compose.Sum
+import DeBruijnSSA.BinSyntax.Typing.Region.Compose
+
+namespace BinSyntax
+
+variable [Φ: EffInstSet φ (Ty α) ε] [PartialOrder α] [SemilatticeSup ε] [OrderBot ε]
+
+namespace Region
+
+open Term.Eqv
+
+def Eqv.distl {A B C : Ty α} {Γ : Ctx α ε} {L : LCtx α}
+  : Eqv φ (⟨(A.prod B).coprod (A.prod C), ⊥⟩::Γ) (A.prod (B.coprod C)::L) :=
+  coprod (A ⋊ inj_l) (A ⋊ inj_r)
+
+def Eqv.distl_inv {A B C : Ty α} {Γ : Ctx α ε} {L : LCtx α}
+  : Eqv φ (⟨A.prod (B.coprod C), ⊥⟩::Γ) ((A.prod B).coprod (A.prod C)::L) :=
+  let2 (var 0 Ctx.Var.shead) $
+  case (var 0 Ctx.Var.shead)
+    (ret $ inl (pair (var 2 (by simp)) (var 0 Ctx.Var.shead)))
+    (ret $ inr (pair (var 2 (by simp)) (var 0 Ctx.Var.shead)))
+
+theorem Eqv.Pure.distl {A B C : Ty α} {Γ : Ctx α ε} {L : LCtx α}
+  : (distl (φ := φ) (A := A) (B := B) (C := C) (Γ := Γ) (L := L)).Pure := sorry
+
+theorem Eqv.Pure.distl_inv {A B C : Ty α} {Γ : Ctx α ε} {L : LCtx α}
+  : (distl_inv (φ := φ) (A := A) (B := B) (C := C) (Γ := Γ) (L := L)).Pure := sorry
+
+-- TODO: dist isomorphism
+
+-- TODO: "naturality"
+
+def Eqv.control {A B : Ty α} {Γ : Ctx α ε} {L : LCtx α}
+  : Eqv φ (⟨A.coprod B, ⊥⟩::Γ) (B::A::L) :=
+  case (var 0 Ctx.Var.shead)
+    (br 1 (var 0 (by simp)) ⟨by simp, le_refl _⟩)
+    (ret (var 0 (by simp)))
+
+def Eqv.fixpoint {A B : Ty α} {Γ : Ctx α ε} {L : LCtx α} (f : Eqv φ (⟨A, ⊥⟩::Γ) ((B.coprod A)::L))
+  : Eqv φ (⟨A, ⊥⟩::Γ) (B::L) := cfg [A] nil (λ| ⟨0, _⟩ => f.vwk1.lwk1 ;; control)
+
+theorem Eqv.fixpoint_iter {A B : Ty α} {Γ : Ctx α ε} {L : LCtx α}
+  (f : Eqv φ (⟨A, ⊥⟩::Γ) ((B.coprod A)::L))
+  : fixpoint f = f ;; coprod nil (fixpoint f) := sorry
+
+theorem Eqv.fixpoint_naturality {A B C : Ty α} {Γ : Ctx α ε} {L : LCtx α}
+  (f : Eqv φ (⟨A, ⊥⟩::Γ) ((B.coprod A)::L))
+  (g : Eqv φ (⟨B, ⊥⟩::Γ) (C::L))
+  : fixpoint (f ;; sum g nil) = (fixpoint f) ;; g := sorry
+
+theorem Eqv.fixpoint_dinaturality {A B C : Ty α} {Γ : Ctx α ε} {L : LCtx α}
+  (f : Eqv φ (⟨A, ⊥⟩::Γ) ((B.coprod C)::L))
+  (g : Eqv φ (⟨C, ⊥⟩::Γ) ((B.coprod A)::L))
+  : fixpoint (f ;; coprod inj_l g) = f ;; coprod nil (fixpoint (g ;; coprod inj_l f)) := sorry
+
+theorem Eqv.fixpoint_codiagonal {A B : Ty α} {Γ : Ctx α ε} {L : LCtx α}
+  (f : Eqv φ (⟨A, ⊥⟩::Γ) (((B.coprod A).coprod A)::L))
+  : fixpoint (f ;; coprod nil inj_r) = fixpoint (fixpoint f) := sorry
+
+theorem Eqv.fixpoint_uniformity {A B : Ty α} {Γ : Ctx α ε} {L : LCtx α}
+  (f : Eqv φ (⟨A, ⊥⟩::Γ) ((B.coprod A)::L)) (g : Eqv φ (⟨C, ⊥⟩::Γ) ((B.coprod C)::L))
+  (h : Eqv φ (⟨C, ⊥⟩::Γ) (A::L)) (hh : h.Pure)
+  (hfg : h ;; f = g ;; sum nil h)
+  : h ;; (fixpoint f) = fixpoint g := sorry
+
+theorem Eqv.fixpoint_strong_left {X A B : Ty α} {Γ : Ctx α ε} {L : LCtx α}
+  (f : Eqv φ (⟨A, ⊥⟩::Γ) ((B.coprod A)::L))
+  : X ⋊ fixpoint f = fixpoint (X ⋊ f ;; distl_inv) := sorry
+
+end Region
+
+end BinSyntax
