DeBruijnSSA/BinSyntax/Rewrite/Region/Compose/Product.lean
@@ -1,0 +1,251 @@
+import DeBruijnSSA.BinSyntax.Rewrite.Region.LSubst
+import DeBruijnSSA.BinSyntax.Rewrite.Region.Compose.Seq
+import DeBruijnSSA.BinSyntax.Typing.Region.Compose
+
+namespace BinSyntax
+
+variable [Φ: EffInstSet φ (Ty α) ε] [PartialOrder α] [SemilatticeSup ε] [OrderBot ε]
+
+namespace Region
+
+open Term.Eqv
+
+def Eqv.rtimes {tyIn tyOut : Ty α} {Γ : Ctx α ε} {L : LCtx α}
+  (tyLeft : Ty α) (r : Eqv φ (⟨tyIn, ⊥⟩::Γ) (tyOut::L))
+  : Eqv φ (⟨tyLeft.prod tyIn, ⊥⟩::Γ) ((tyLeft.prod tyOut)::L)
+  := Eqv.let2 (var 0 Ctx.Var.shead) $
+  r.vwk1.vwk1 ;;
+  ret (pair (var 1 (by simp)) (var 0 (by simp)))
+
+infixl:70 " ⋊ "  => Eqv.rtimes
+
+theorem Eqv.Pure.rtimes {tyIn tyOut : Ty α} {Γ : Ctx α ε} {L : LCtx α}
+  (tyLeft : Ty α) {r : Eqv φ (⟨tyIn, ⊥⟩::Γ) (tyOut::L)}
+  : Eqv.Pure r → Eqv.Pure (tyLeft ⋊ r) := sorry
+
+def Eqv.braid {left right : Ty α} {Γ : Ctx α ε} {L : LCtx α}
+  : Eqv φ (⟨left.prod right, ⊥⟩::Γ) ((right.prod left)::L)
+  := Eqv.let2 (var 0 Ctx.Var.shead) $
+  ret (pair (var 0 (by simp)) (var 1 (by simp)))
+
+theorem Eqv.Pure.braid {left right : Ty α} {Γ : Ctx α ε} {L : LCtx α}
+  : Eqv.Pure (Eqv.braid (φ := φ) (left := left) (right := right) (Γ := Γ) (L := L)) := sorry
+
+theorem Eqv.repack {left right : Ty α} {rest : Ctx α ε} {targets : LCtx α}
+  : Eqv.let2 (var 0 ⟨by simp, le_refl _⟩)
+    (Eqv.ret (pair (var 1 (by simp)) (var 0 (by simp))))
+  = Eqv.nil (φ := φ) (ty := left.prod right) (rest := rest) (targets := targets) := by
+  rw [<-let1_0_nil, <-let2_eta, let1_beta]
+  rfl
+
+theorem Eqv.braid_braid {left right : Ty α}
+  : Eqv.braid ;; Eqv.braid
+  = (Eqv.nil (φ := φ) (ty := left.prod right) (rest := rest) (targets := targets)) := by
+  stop
+  simp only [
+    braid, let2_seq, vwk1, vwk_let2, wk_var, wk_pair, Nat.liftWk, vwk_ret, Ctx.InS.liftn₂,
+    Nat.liftnWk, Nat.one_lt_ofNat, Nat.ofNat_pos, ↓reduceIte, ret_seq, vsubst_let2,
+    subst_pair, subst_var, Term.Subst.InS.get_0_subst0, let2_pair, let1_beta, vsubst_vsubst
+  ]
+  apply Eqv.repack
+
+theorem Eqv.rtimes_nil {ty : Ty α} {Γ : Ctx α ε} {L : LCtx α}
+  (tyLeft : Ty α)
+  : tyLeft ⋊ Eqv.nil = (Eqv.nil (φ := φ) (ty := tyLeft.prod ty) (rest := Γ) (targets := L)) := by
+  simp only [rtimes, nil_vwk1, nil_seq, repack]
+
+theorem Eqv.rtimes_seq {A B C : Ty α} {Γ : Ctx α ε} {L : LCtx α}
+  (tyLeft : Ty α) (r : Eqv φ (⟨A, ⊥⟩::Γ) (B::L)) (s : Eqv φ (⟨B, ⊥⟩::Γ) (C::L))
+  : tyLeft ⋊ (r ;; s) = (tyLeft ⋊ r) ;; (tyLeft ⋊ s) := by
+  stop
+  apply Eq.symm
+  rw [rtimes, rtimes, let2_seq, seq_assoc, ret_seq]
+  simp only [
+    vwk1, vwk_let2, wk_var, Nat.liftWk, vsubst_let2, vwk_vwk, Ctx.InS.liftn₂_comp_liftn₂,
+    subst_pair, subst_var, Term.Subst.InS.get_0_subst0, let2_pair, let1_beta,
+    vsubst_vsubst
+  ]
+  apply congrArg
+  rw [vwk1_seq, vwk1_seq, seq_assoc]
+  congr 1
+  . simp [vwk1, vwk_vwk]
+  . sorry
+
+def Eqv.ltimes {tyIn tyOut : Ty α} {Γ : Ctx α ε} {L : LCtx α}
+  (r : Eqv φ (⟨tyIn, ⊥⟩::Γ) (tyOut::L)) (tyRight : Ty α)
+  : Eqv φ (⟨tyIn.prod tyRight, ⊥⟩::Γ) ((tyOut.prod tyRight)::L)
+  := Eqv.braid ;; tyRight ⋊ r ;; Eqv.braid
+
+infixl:70 " ⋉ "  => Eqv.ltimes
+
+theorem Eqv.Pure.ltimes {tyIn tyOut : Ty α} {Γ : Ctx α ε} {L : LCtx α}
+  {r : Eqv φ (⟨tyIn, ⊥⟩::Γ) (tyOut::L)} (hr : r.Pure) (tyRight : Ty α)
+  : Pure (r ⋉ tyRight) := seq (seq braid (hr.rtimes _)) braid
+
+theorem Eqv.braid_rtimes_braid {Γ : Ctx α ε} {L : LCtx α}
+  (r : Eqv φ (⟨A, ⊥⟩::Γ) (B::L))
+  : Eqv.braid ;; C ⋊ r ;; Eqv.braid = r ⋉ C
+  := rfl
+
+theorem Eqv.braid_ltimes {Γ : Ctx α ε} {L : LCtx α}
+  (r : Eqv φ (⟨A, ⊥⟩::Γ) (B::L))
+  : Eqv.braid ;; r ⋉ C = C ⋊ r ;; Eqv.braid
+  := by rw [<-braid_rtimes_braid, <-seq_assoc, <-seq_assoc, braid_braid, nil_seq]
+
+theorem Eqv.braid_ltimes_braid {Γ : Ctx α ε} {L : LCtx α}
+  (r : Eqv φ (⟨A, ⊥⟩::Γ) (B::L))
+  : Eqv.braid ;; r ⋉ C ;; Eqv.braid = C ⋊ r
+  := by rw [
+    ltimes, seq_assoc, seq_assoc, braid_braid, seq_assoc, seq_nil, <-seq_assoc, braid_braid, nil_seq]
+
+theorem Eqv.braid_rtimes {Γ : Ctx α ε} {L : LCtx α}
+  (r : Eqv φ (⟨A, ⊥⟩::Γ) (B::L))
+  : Eqv.braid ;; C ⋊ r = r ⋉ C ;; Eqv.braid
+  := by rw [<-braid_ltimes_braid, <-seq_assoc, <-seq_assoc, braid_braid, nil_seq]
+
+theorem Eqv.ltimes_nil {ty : Ty α} {Γ : Ctx α ε} {L : LCtx α}
+  : Eqv.nil ⋉ tyRight = (Eqv.nil (φ := φ) (ty := ty.prod tyRight) (rest := Γ) (targets := L))
+  := by rw [<-braid_rtimes_braid, rtimes_nil, seq_nil, braid_braid]
+
+theorem Eqv.ltimes_seq {A B C : Ty α} {Γ : Ctx α ε} {L : LCtx α}
+  (r : Eqv φ (⟨A, ⊥⟩::Γ) (B::L)) (s : Eqv φ (⟨B, ⊥⟩::Γ) (C::L))
+  : (r ;; s) ⋉ tyRight = (r ⋉ tyRight) ;; (s ⋉ tyRight) := by
+  simp only [<-braid_rtimes_braid, rtimes_seq, seq_assoc]
+  rw [<-seq_assoc braid braid, braid_braid, nil_seq]
+
+def Eqv.runit {ty : Ty α} {Γ : Ctx α ε} {L : LCtx α}
+  : Eqv φ (⟨ty.prod Ty.unit, ⊥⟩::Γ) (ty::L)
+  := let2 (var 0 Ctx.Var.shead) (ret $ var 1 (by simp))
+
+def Eqv.runit_inv {ty : Ty α} {Γ : Ctx α ε} {L : LCtx α}
+  : Eqv φ (⟨ty, ⊥⟩::Γ) (ty.prod Ty.unit::L)
+  := ret $ (pair (var 0 Ctx.Var.shead) (unit _))
+
+theorem Eqv.Pure.runit {ty : Ty α} {Γ : Ctx α ε} {L : LCtx α}
+  : (runit (φ := φ) (ty := ty) (Γ := Γ) (L := L)).Pure := sorry
+
+theorem Eqv.Pure.runit_inv {ty : Ty α} {Γ : Ctx α ε} {L : LCtx α}
+  : (runit_inv (φ := φ) (ty := ty) (Γ := Γ) (L := L)).Pure := sorry
+
+theorem Eqv.runit_runit_inv_helper {ty : Ty α} {Γ : Ctx α ε} {L : LCtx α}
+  : runit (φ := φ) (ty := ty) (Γ := Γ) (L := L) ;; runit_inv
+  = let2 (var 0 ⟨by simp, le_refl _⟩)
+    (let1 (unit ⊥) (ret $ pair (var 2 (by simp)) (var 0 (by simp)))) := by
+  rw [let1_beta]
+  rfl
+
+theorem Eqv.runit_runit_inv {ty : Ty α} {Γ : Ctx α ε} {L : LCtx α}
+  : runit (φ := φ) (ty := ty) (Γ := Γ) (L := L) ;; runit_inv = nil := by
+  rw [runit_runit_inv_helper, terminal _ (var 0 (by simp)), let1_beta]
+  apply repack
+
+theorem Eqv.runit_inv_runit {ty : Ty α} {Γ : Ctx α ε} {L : LCtx α}
+  : runit_inv (φ := φ) (ty := ty) (Γ := Γ) (L := L) ;; runit = nil := by
+  stop
+  simp only [runit_inv, runit, ret_seq]
+  rw [vwk1, vwk_let2, vsubst_let2, wk_var, subst_var]
+  simp only [Nat.liftWk_zero, Term.Subst.InS.get_0_subst0, Set.mem_setOf_eq]
+  rw [let2_pair, let1_beta, let1_beta]
+  rfl
+
+theorem Eqv.ltimes_runit {ty : Ty α} {Γ : Ctx α ε} {L : LCtx α}
+  (r : Eqv φ (⟨A, ⊥⟩::Γ) (B::L))
+  : r ⋉ Ty.unit ;; runit = runit ;; r := sorry
+
+def Eqv.lunit {ty : Ty α} {Γ : Ctx α ε} {L : LCtx α}
+  : Eqv φ (⟨Ty.unit.prod ty, ⊥⟩::Γ) (ty::L)
+  := let2 (var 0 Ctx.Var.shead) (ret $ var 0 (by simp))
+
+def Eqv.lunit_inv {ty : Ty α} {Γ : Ctx α ε} {L : LCtx α}
+  : Eqv φ (⟨ty, ⊥⟩::Γ) (Ty.unit.prod ty::L)
+  := ret $ (pair (unit _) (var 0 Ctx.Var.shead))
+
+theorem Eqv.Pure.lunit {ty : Ty α} {Γ : Ctx α ε} {L : LCtx α}
+  : (lunit (φ := φ) (ty := ty) (Γ := Γ) (L := L)).Pure := sorry
+
+theorem Eqv.Pure.lunit_inv {ty : Ty α} {Γ : Ctx α ε} {L : LCtx α}
+  : (lunit_inv (φ := φ) (ty := ty) (Γ := Γ) (L := L)).Pure := sorry
+
+theorem Eqv.lunit_seq_lunit_inv {ty : Ty α} {Γ : Ctx α ε} {L : LCtx α}
+  : lunit (φ := φ) (ty := ty) (Γ := Γ) (L := L) ;; lunit_inv = nil
+  := sorry
+
+theorem Eqv.lunit_inv_lunit {ty : Ty α} {Γ : Ctx α ε} {L : LCtx α}
+  : lunit_inv (φ := φ) (ty := ty) (Γ := Γ) (L := L) ;; lunit = nil
+  := sorry
+
+-- TODO: braid ;; lunit = runit, lunit_inv ;; braid = runit_inv, and vice versa...
+
+theorem Eqv.rtimes_lunit {ty : Ty α} {Γ : Ctx α ε} {L : LCtx α}
+  (r : Eqv φ (⟨A, ⊥⟩::Γ) (B::L))
+  : Ty.unit ⋊ r ;; lunit = lunit ;; r
+  := sorry
+
+theorem Eqv.Pure.central_left {A A' B B' : Ty α} {Γ : Ctx α ε} {L : LCtx α}
+  {l : Eqv φ (⟨A, ⊥⟩::Γ) (A'::L)}
+  (hl : l.Pure)
+  (r : Eqv φ (⟨B, ⊥⟩::Γ) (B'::L))
+  : (l ⋉ B) ;; (A' ⋊ r) = (A ⋊ r) ;; (l ⋉ B') := sorry
+
+theorem Eqv.Pure.central_right {A A' B B' : Ty α} {Γ : Ctx α ε} {L : LCtx α}
+  (l : Eqv φ (⟨A, ⊥⟩::Γ) (A'::L))
+  {r : Eqv φ (⟨B, ⊥⟩::Γ) (B'::L)}
+  (hr : r.Pure)
+  : (A ⋊ r) ;; (l ⋉ B') = (l ⋉ B) ;; (A' ⋊ r) := by
+  rw [
+    <-braid_rtimes_braid, <-seq_assoc, <-seq_assoc, <-braid_ltimes, seq_assoc Eqv.braid,
+    hr.central_left, <-seq_assoc, braid_rtimes, seq_assoc (l ⋉ B), braid_ltimes,
+    seq_assoc, seq_assoc (A' ⋊ r), braid_braid, seq_nil
+  ]
+
+def Eqv.assoc {A B C : Ty α} {Γ : Ctx α ε} {L : LCtx α}
+  : Eqv φ (⟨(A.prod B).prod C, ⊥⟩::Γ) (A.prod (B.prod C)::L) :=
+  let2 (var 0 ⟨by simp, le_refl _⟩) $
+  let2 (var 1 ⟨by simp, le_refl _⟩) $
+  ret $ pair (var 1 (by simp)) (pair (var 0 (by simp)) (var 2 (by simp)))
+
+def Eqv.assoc_inv {A B C : Ty α} {Γ : Ctx α ε} {L : LCtx α}
+  : Eqv φ (⟨A.prod (B.prod C), ⊥⟩::Γ) ((A.prod B).prod C::L) :=
+  let2 (var 0 ⟨by simp, le_refl _⟩) $
+  let2 (var 0 ⟨by simp, le_refl _⟩) $
+  ret $ pair (pair (var 3 (by simp)) (var 1 (by simp))) (var 0 (by simp))
+
+theorem Eqv.Pure.assoc {A B C : Ty α} {Γ : Ctx α ε} {L : LCtx α}
+  : (assoc (φ := φ) (A := A) (B := B) (C := C) (Γ := Γ) (L := L)).Pure := sorry
+
+theorem Eqv.Pure.assoc_inv {A B C : Ty α} {Γ : Ctx α ε} {L : LCtx α}
+  : (assoc_inv (φ := φ) (A := A) (B := B) (C := C) (Γ := Γ) (L := L)).Pure := sorry
+
+theorem Eqv.assoc_assoc_inv {A B C : Ty α} {Γ : Ctx α ε} {L : LCtx α}
+  : assoc (φ := φ) (A := A) (B := B) (C := C) (Γ := Γ) (L := L) ;; assoc_inv = nil
+  := sorry
+
+theorem Eqv.assoc_inv_assoc {A B C : Ty α} {Γ : Ctx α ε} {L : LCtx α}
+  : assoc_inv (φ := φ) (A := A) (B := B) (C := C) (Γ := Γ) (L := L) ;; assoc = nil
+  := sorry
+
+theorem Eqv.assoc_left_nat {A B C A' : Ty α} {Γ : Ctx α ε} {L : LCtx α}
+  (l : Eqv φ (⟨A, ⊥⟩::Γ) (A'::L))
+  : (l ⋉ B) ⋉ C ;; assoc = assoc ;; l ⋉ (B.prod C) := sorry
+
+theorem Eqv.assoc_mid_nat {A B C B' : Ty α} {Γ : Ctx α ε} {L : LCtx α}
+  (m : Eqv φ (⟨B, ⊥⟩::Γ) (B'::L))
+  : (A ⋊ m) ⋉ C ;; assoc = assoc ;; A ⋊ (m ⋉ C) := sorry
+
+theorem Eqv.assoc_right_nat {A B C C' : Ty α} {Γ : Ctx α ε} {L : LCtx α}
+  (r : Eqv φ (⟨C, ⊥⟩::Γ) (C'::L))
+  : (A.prod B) ⋊ r ;; assoc = assoc ;; A ⋊ (B ⋊ r) := sorry
+
+theorem Eqv.triangle {X Y : Ty α} {Γ : Ctx α ε} {L : LCtx α}
+  : assoc (φ := φ) (Γ := Γ) (L := L) (A := X) (B := Ty.unit) (C := Y) ;; X ⋊ lunit
+  = runit ⋉ Y := sorry
+
+theorem Eqv.pentagon {W X Y Z : Ty α} {Γ : Ctx α ε} {L : LCtx α}
+  : assoc (φ := φ) (Γ := Γ) (L := L) (A := W.prod X) (B := Y) (C := Z) ;; assoc
+  = assoc ⋉ Z ;; assoc ;; W ⋊ assoc
+  := sorry
+
+theorem Eqv.hexagon {X Y Z : Ty α} {Γ : Ctx α ε} {L : LCtx α}
+  : assoc (φ := φ) (Γ := Γ) (L := L) (A := X) (B := Y) (C := Z) ;; braid ;; assoc
+  = braid ⋉ Z ;; assoc ;; Y ⋊ braid
+  := sorry
