DeBruijnSSA/BinSyntax/Rewrite/Region/Compose/Seq.lean
@@ -1,0 +1,262 @@
+import DeBruijnSSA.BinSyntax.Rewrite.Region.LSubst
+import DeBruijnSSA.BinSyntax.Typing.Region.Compose
+
+namespace BinSyntax
+
+variable [Φ: EffInstSet φ (Ty α) ε] [PartialOrder α] [SemilatticeSup ε] [OrderBot ε]
+
+namespace Region
+
+abbrev Eqv.ret {tyIn tyOut : Ty α} {rest: Ctx α ε} {targets : LCtx α}
+  (t : Term.Eqv φ (⟨tyIn, ⊥⟩::rest) ⟨tyOut, ⊥⟩)
+  : Eqv φ (⟨tyIn, ⊥⟩::rest) (tyOut::targets)
+  := Quotient.liftOn t (λt => ⟦InS.ret t⟧) (λ_ _ h => Quotient.sound $ InS.br_congr _ h (by simp))
+
+theorem Eqv.vwk_ret {tyIn tyOut : Ty α} {rest: Ctx α ε} {targets : LCtx α}
+  (ρ : Ctx.InS (⟨tyIn, ⊥⟩::rest') _)
+  (t : Term.Eqv φ (⟨tyIn, ⊥⟩::rest) ⟨tyOut, ⊥⟩)
+  : (Eqv.ret (targets := targets) t).vwk ρ = Eqv.ret (t.wk ρ) := by
+  induction t using Quotient.inductionOn
+  rfl
+
+theorem Eqv.vwk1_ret {tyIn tyOut : Ty α} {rest: Ctx α ε} {targets : LCtx α}
+  (t : Term.Eqv φ (⟨tyIn, ⊥⟩::rest) ⟨tyOut, ⊥⟩)
+  : (Eqv.ret (targets := targets) t).vwk1 (inserted := inserted)
+  = Eqv.ret (t.wk ⟨Nat.liftWk Nat.succ, by simp⟩) := by
+  induction t using Quotient.inductionOn
+  rfl
+
+theorem Eqv.vsubst_ret {tyIn tyOut : Ty α} {rest: Ctx α ε} {targets : LCtx α}
+  (σ : Term.Subst.Eqv φ (⟨tyIn, ⊥⟩::Γ) _)
+  (t : Term.Eqv φ (⟨tyIn, ⊥⟩::rest) ⟨tyOut, ⊥⟩)
+  : (Eqv.ret (targets := targets) t).vsubst σ = Eqv.ret (t.subst σ) := by
+  induction σ using Quotient.inductionOn
+  induction t using Quotient.inductionOn
+  rfl
+
+abbrev Eqv.nil {ty : Ty α} {rest: Ctx α ε} {targets : LCtx α}
+  : Eqv φ (⟨ty, ⊥⟩::rest) (ty::targets) := ⟦InS.nil⟧
+
+@[simp]
+theorem Eqv.nil_vwk_lift (ρ : Ctx.InS rest _)
+  : (Eqv.nil (φ := φ) (ty := ty) (rest := rest') (targets := targets)).vwk (ρ.lift h) = Eqv.nil
+  := rfl
+
+@[simp]
+theorem Eqv.nil_vwk_liftn₂ (ρ : Ctx.InS rest _)
+  : (Eqv.nil (φ := φ) (ty := ty) (rest := (head'::rest')) (targets := targets)).vwk (ρ.liftn₂ h h')
+  = Eqv.nil
+  := rfl
+
+theorem Eqv.nil_vwk1 {Γ : Ctx α ε} {L : LCtx α}
+  : (Eqv.nil (φ := φ) (ty := ty) (rest := Γ) (targets := L)).vwk1 (inserted := inserted)
+  = Eqv.nil := rfl
+
+theorem Eqv.let1_0_nil
+  : Eqv.let1 (Term.Eqv.var 0 ⟨by simp, le_refl _⟩) Eqv.nil
+  = Eqv.nil (φ := φ) (ty := ty) (rest := rest) (targets := targets)
+  := by rw [let1_beta]; rfl
+
+def Wf.lsubst0 {Γ : Ctx α ε} {L : LCtx α} {r : Region φ} (hr : r.Wf (⟨A, ⊥⟩::Γ) L)
+  : r.lsubst0.Wf Γ (A::L) L
+  := Fin.cases hr (λi => Wf.br ⟨i.prop, le_refl _⟩ (by simp))
+
+def InS.lsubst0 {A : Ty α} {Γ : Ctx α ε} {L : LCtx α} (r : InS φ (⟨A, ⊥⟩::Γ) L)
+  : Subst.InS φ Γ (A::L) L
+  := ⟨(r : Region φ).lsubst0, r.prop.lsubst0⟩
+
+theorem InS.lsubst0_congr {A : Ty α} {Γ : Ctx α ε} {L : LCtx α} {r r' : InS φ (⟨A, ⊥⟩::Γ) L}
+  (h : r ≈ r') : InS.lsubst0 r ≈ InS.lsubst0 r'
+  := sorry
+
+def Eqv.lsubst0 {A : Ty α} {Γ : Ctx α ε} {L : LCtx α} (r : Eqv φ (⟨A, ⊥⟩::Γ) L)
+  : Subst.Eqv φ Γ (A::L) L
+  := Quot.liftOn r (λr => ⟦InS.lsubst0 r⟧) (λ_ _ h => Quotient.sound $ InS.lsubst0_congr h)
+
+theorem InS.alpha0_congr {A B : Ty α} {Γ : Ctx α ε} {L : LCtx α} {r r' : InS φ (⟨A, ⊥⟩::Γ) (B::L)}
+  (h : r ≈ r') : InS.alpha0 r ≈ InS.alpha0 r'
+  := sorry
+
+def Eqv.alpha0 {A B : Ty α} {Γ : Ctx α ε} {L : LCtx α} (r : Eqv φ (⟨A, ⊥⟩::Γ) (B::L))
+  : Subst.Eqv φ Γ (A::L) (B::L)
+  := Quot.liftOn r (λr => ⟦InS.alpha0 r⟧) (λ_ _ h => Quotient.sound $ InS.alpha0_congr h)
+
+@[simp]
+theorem Eqv.alpha0_quot {A B : Ty α} {Γ : Ctx α ε} {L : LCtx α} (r : InS φ (⟨A, ⊥⟩::Γ) (B::L))
+  : Eqv.alpha0 ⟦r⟧ = ⟦InS.alpha0 r⟧ := rfl
+
+theorem Eqv.vlift_alpha0 {A B : Ty α} {Γ : Ctx α ε} {L : LCtx α} (r : Eqv φ (⟨A, ⊥⟩::Γ) (B::L))
+  : (Eqv.alpha0 r).vlift = Eqv.alpha0 (r.vwk1 (inserted := X)) := by
+  induction r using Quotient.inductionOn;
+  rw [alpha0_quot, Subst.Eqv.vlift_quot, InS.vlift_alpha0]
+  rfl
+
+def Eqv.seq {A B C : Ty α} {Γ : Ctx α ε} {L : LCtx α}
+  (left : Eqv φ (⟨A, ⊥⟩::Γ) (B::L)) (right : Eqv φ (⟨B, ⊥⟩::Γ) (C::L)) : Eqv φ (⟨A, ⊥⟩::Γ) (C::L)
+  := left.lsubst right.vwk1.alpha0
+
+instance Eqv.instHAppend {A B C : Ty α} {Γ : Ctx α ε} {L : LCtx α}
+  : HAppend (Eqv φ (⟨A, ⊥⟩::Γ) (B::L)) (Eqv φ (⟨B, ⊥⟩::Γ) (C::L)) (Eqv φ (⟨A, ⊥⟩::Γ) (C::L)) where
+  hAppend := Eqv.seq
+
+infixl:65 " ;; "  => Eqv.seq
+
+theorem Eqv.seq_def {A B C : Ty α} {Γ : Ctx α ε} {L : LCtx α}
+  (left : Eqv φ (⟨A, ⊥⟩::Γ) (B::L)) (right : Eqv φ (⟨B, ⊥⟩::Γ) (C::L))
+  : left ;; right = left.lsubst right.vwk1.alpha0 := rfl
+
+@[simp]
+theorem Eqv.seq_quot {A B C : Ty α} {Γ : Ctx α ε} {L : LCtx α}
+  (left : InS φ (⟨A, ⊥⟩::Γ) (B::L)) (right : InS φ (⟨B, ⊥⟩::Γ) (C::L))
+  : ⟦left⟧ ;; ⟦right⟧ = ⟦left ++ right⟧
+  := rfl
+
+@[simp]
+theorem InS.append_q {A B C : Ty α} {Γ : Ctx α ε} {L : LCtx α}
+  (left : InS φ (⟨A, ⊥⟩::Γ) (B::L)) (right : InS φ (⟨B, ⊥⟩::Γ) (C::L))
+  : left.q ++ right.q = (left ++ right).q
+  := rfl
+
+@[simp]
+theorem InS.seq_q {A B C : Ty α} {Γ : Ctx α ε} {L : LCtx α}
+  (left : InS φ (⟨A, ⊥⟩::Γ) (B::L)) (right : InS φ (⟨B, ⊥⟩::Γ) (C::L))
+  : left.q ;; right.q = (left ++ right).q
+  := rfl
+
+@[simp]
+theorem Eqv.seq_nil {A B : Ty α} {Γ : Ctx α ε} {L : LCtx α}
+  (left : Eqv φ (⟨A, ⊥⟩::Γ) (B::L))
+  : left ;; Eqv.nil = left := by
+  induction left using Quotient.inductionOn;
+  simp [nil]
+
+@[simp]
+theorem Eqv.nil_seq {A B : Ty α} {Γ : Ctx α ε} {L : LCtx α}
+  (left : Eqv φ (⟨A, ⊥⟩::Γ) (B::L))
+  : Eqv.nil ;; left = left := by
+  induction left using Quotient.inductionOn;
+  simp [nil]
+
+theorem Eqv.seq_assoc {A B C D : Ty α} {Γ : Ctx α ε} {L : LCtx α}
+  (left : Eqv φ (⟨A, ⊥⟩::Γ) (B::L))
+  (middle : Eqv φ (⟨B, ⊥⟩::Γ) (C::L))
+  (right : Eqv φ (⟨C, ⊥⟩::Γ) (D::L))
+  : (left ;; middle) ;; right = left ;; (middle ;; right) := by
+  induction left using Quotient.inductionOn;
+  induction middle using Quotient.inductionOn;
+  induction right using Quotient.inductionOn;
+  simp [InS.append_assoc]
+
+theorem Eqv.ret_seq {A B C : Ty α} {Γ : Ctx α ε} {L : LCtx α}
+  (a : Term.Eqv φ (⟨A, ⊥⟩::Γ) ⟨B, ⊥⟩)
+  (r : Eqv φ (⟨B, ⊥⟩::Γ) (C::L))
+  : (Eqv.ret a) ;; r = r.vwk1.vsubst a.subst0 := by
+  induction a using Quotient.inductionOn;
+  induction r using Quotient.inductionOn;
+  simp only [ret, seq_def, vwk1_quot, alpha0_quot, lsubst_quot, vsubst_quot]
+  rfl
+
+theorem Eqv.ret_seq_let {A B C : Ty α} {Γ : Ctx α ε} {L : LCtx α}
+  (a : Term.Eqv φ (⟨A, ⊥⟩::Γ) ⟨B, ⊥⟩)
+  (r : Eqv φ (⟨B, ⊥⟩::Γ) (C::L))
+  : (Eqv.ret a) ;; r = let1 a r.vwk1 := by rw [ret_seq, let1_beta]
+
+theorem Eqv.let1_seq {Γ : Ctx α ε} {L : LCtx α}
+  (a : Term.Eqv φ (⟨A, ⊥⟩::Γ) ⟨X, e⟩)
+  (r : Eqv φ (⟨X, ⊥⟩::⟨A, ⊥⟩::Γ) (B::L)) (s : Eqv φ (⟨B, ⊥⟩::Γ) (C::L))
+  : (Eqv.let1 a r) ;; s = Eqv.let1 a (r ;; s.vwk1) := by
+  simp only [seq_def, lsubst_let1, vlift_alpha0]
+
+theorem Eqv.let2_seq {Γ : Ctx α ε} {L : LCtx α}
+  (a : Term.Eqv φ (⟨A, ⊥⟩::Γ) ⟨X.prod Y, e⟩)
+  (r : Eqv φ (⟨Y, ⊥⟩::⟨X, ⊥⟩::⟨A, ⊥⟩::Γ) (C::L)) (s : Eqv φ (⟨C, ⊥⟩::Γ) (D::L))
+  : (Eqv.let2 a r) ;; s = Eqv.let2 a (r ;; s.vwk1.vwk1) := by
+  simp only [seq_def, lsubst_let2, Subst.Eqv.vliftn₂_eq_vlift_vlift, vlift_alpha0]
+
+theorem Eqv.case_seq {Γ : Ctx α ε} {L : LCtx α}
+  (a : Term.Eqv φ (⟨A, ⊥⟩::Γ) ⟨X.coprod Y, e⟩)
+  (r : Eqv φ (⟨X, ⊥⟩::⟨A, ⊥⟩::Γ) (B::L)) (s : Eqv φ (⟨Y, ⊥⟩::⟨A, ⊥⟩::Γ) (B::L))
+  (t : Eqv φ (⟨B, ⊥⟩::Γ) (C::L))
+  : (Eqv.case a r s) ;; t = Eqv.case a (r ;; t.vwk1) (s ;; t.vwk1) := by
+  simp only [seq_def, lsubst_case, vlift_alpha0]
+
+theorem Eqv.vwk_lift_seq {A B C : Ty α} {Γ Δ : Ctx α ε} {L : LCtx α}
+  (ρ : Ctx.InS Γ Δ)
+  (left : Eqv φ (⟨A, ⊥⟩::Δ) (B::L))
+  (right : Eqv φ (⟨B, ⊥⟩::Δ) (C::L))
+  : (left ;; right).vwk (ρ.lift (le_refl _))
+  = left.vwk (ρ.lift (le_refl _)) ;; right.vwk (ρ.lift (le_refl _)) := by
+  induction left using Quotient.inductionOn;
+  induction right using Quotient.inductionOn;
+  sorry
+
+theorem Eqv.vwk_liftn₂_seq {A B C : Ty α} {Γ Δ : Ctx α ε} {L : LCtx α}
+  (ρ : Ctx.InS Γ Δ)
+  (left : Eqv φ (⟨A, ⊥⟩::X::Δ) (B::L))
+  (right : Eqv φ (⟨B, ⊥⟩::X::Δ) (C::L))
+  : (left ;; right).vwk (ρ.liftn₂ (le_refl _) (le_refl _))
+  = left.vwk (ρ.liftn₂ (le_refl _) (le_refl _)) ;; right.vwk (ρ.liftn₂ (le_refl _) (le_refl _))
+  := by simp only [<-Ctx.InS.lift_lift, vwk_lift_seq]
+
+theorem Eqv.vwk1_seq {A B C : Ty α} {Γ : Ctx α ε} {L : LCtx α}
+  (left : Eqv φ (⟨A, ⊥⟩::Γ) (B::L))
+  (right : Eqv φ (⟨B, ⊥⟩::Γ) (C::L))
+  : (left ;; right).vwk1 (inserted := inserted)
+  = left.vwk1 ;; right.vwk1 := vwk_lift_seq ⟨Nat.succ, (by simp)⟩ left right
+
+theorem Eqv.vsubst_lift_seq {A B C : Ty α} {Γ Δ : Ctx α ε} {L : LCtx α}
+  (σ : Term.Subst.Eqv φ Γ Δ)
+  (left : Eqv φ (⟨A, ⊥⟩::Δ) (B::L))
+  (right : Eqv φ (⟨B, ⊥⟩::Δ) (C::L))
+  : (left ;; right).vsubst (σ.lift (le_refl _))
+  = left.vsubst (σ.lift (le_refl _)) ;; right.vsubst (σ.lift (le_refl _)) := by
+  induction left using Quotient.inductionOn;
+  induction right using Quotient.inductionOn;
+  sorry
+
+theorem Eqv.vsubst_liftn₂_seq {A B C : Ty α} {Γ Δ : Ctx α ε} {L : LCtx α}
+  (σ : Term.Subst.Eqv φ Γ Δ)
+  (left : Eqv φ (⟨A, ⊥⟩::X::Δ) (B::L))
+  (right : Eqv φ (⟨B, ⊥⟩::X::Δ) (C::L))
+  : (left ;; right).vsubst (σ.liftn₂ (le_refl _) (le_refl _))
+  = left.vsubst (σ.liftn₂ (le_refl _) (le_refl _)) ;; right.vsubst (σ.liftn₂ (le_refl _) (le_refl _))
+  := by stop simp only [<-Term.Subst.InS.lift_lift, vsubst_lift_seq]
+
+-- TODO: centrality lore...
+
+-- inductive PureTree : (Γ : ℕ → ε) → Region φ → Prop
+--   | ret a : PureTree Γ (ret a)
+--   | case e l r
+--     : e.effect Γ = ⊥
+--       → PureTree (Nat.liftBot Γ) l
+--       → PureTree (Nat.liftBot Γ) r
+--       → PureTree Γ (case e l r)
+--   | let1 e r
+--     : e.effect Γ = ⊥
+--       → PureTree (Nat.liftBot Γ) r
+--       → PureTree Γ (let1 e r)
+--   | let2 e r
+--     : e.effect Γ = ⊥
+--       → PureTree (Nat.liftBot Γ) r
+--       → PureTree Γ (let2 e r)
+
+-- def InS.PureTree {Γ : Ctx α ε} {L : LCtx α} (r : InS φ Γ L) : Prop
+--   := Region.PureTree (φ := φ) Γ.effect r
+
+def Eqv.Pure {Γ : Ctx α ε} {L : LCtx α} (r : Eqv φ (⟨A, ⊥⟩::Γ) (B::L)) : Prop
+  := ∃a : Term.Eqv φ (⟨A, ⊥⟩::Γ) ⟨B, ⊥⟩, r = ret a
+
+-- TODO: ret, case, let1, let2
+
+-- TODO: closed under vwk, lwk (lift), vsubst, lsubst (pure), ltimes, rtimes...
+
+theorem Eqv.Pure.nil {Γ : Ctx α ε} {L : LCtx α}
+  : Eqv.Pure (Eqv.nil (φ := φ) (ty := ty) (rest := Γ) (targets := L)) := sorry
+
+theorem Eqv.Pure.seq {Γ : Ctx α ε} {L : LCtx α}
+  {r : Eqv φ (⟨A, ⊥⟩::Γ) (B::L)} {s : Eqv φ (⟨B, ⊥⟩::Γ) (C::L)}
+  (hr : r.Pure) (hs : s.Pure) : (r ;; s).Pure := sorry
+
+-- TODO: ret, case, let1, let2
+
+-- TODO: closed under vwk, lwk (lift), vsubst, lsubst (pure), append...
