DeBruijnSSA/BinSyntax/Rewrite/Region/Compose/Sum.lean
@@ -1,0 +1,234 @@
+import DeBruijnSSA.BinSyntax.Rewrite.Region.LSubst
+import DeBruijnSSA.BinSyntax.Rewrite.Region.Compose.Seq
+import DeBruijnSSA.BinSyntax.Typing.Region.Compose
+
+namespace BinSyntax
+
+variable [Φ: EffInstSet φ (Ty α) ε] [PartialOrder α] [SemilatticeSup ε] [OrderBot ε]
+
+namespace Region
+
+open Term.Eqv
+
+def Eqv.coprod {A B C : Ty α} {Γ : Ctx α ε} {L : LCtx α}
+  (l : Eqv φ (⟨A, ⊥⟩::Γ) (C::L)) (r : Eqv φ (⟨B, ⊥⟩::Γ) (C::L))
+  : Eqv φ (⟨A.coprod B, ⊥⟩::Γ) (C::L)
+  := case (var 0 Ctx.Var.shead) l.vwk1 r.vwk1
+
+theorem Eqv.Pure.coprod {A B C : Ty α} {Γ : Ctx α ε} {L : LCtx α}
+  {l : Eqv φ (⟨A, ⊥⟩::Γ) (C::L)} (hl : l.Pure)
+  {r : Eqv φ (⟨B, ⊥⟩::Γ) (C::L)} (hr : r.Pure)
+  : (coprod l r).Pure := sorry
+
+theorem Eqv.coprod_seq {A B C D : Ty α} {Γ : Ctx α ε} {L : LCtx α}
+  (l : Eqv φ (⟨A, ⊥⟩::Γ) (C::L)) (r : Eqv φ (⟨B, ⊥⟩::Γ) (C::L)) (s : Eqv φ (⟨C, ⊥⟩::Γ) (D::L))
+  : (coprod l r) ;; s = coprod (l ;; s) (r ;; s)
+  := by simp [coprod, case_seq, vwk1_seq]
+
+def Eqv.join {Γ : Ctx α ε} {L : LCtx α} {A : Ty α}
+  : Eqv φ (⟨A.coprod A, ⊥⟩::Γ) (A::L)
+  := coprod nil nil
+
+def Eqv.zero {Γ : Ctx α ε} {L : LCtx α} {A : Ty α}
+  : Eqv φ (⟨Ty.empty, ⊥⟩::Γ) (A::L)
+  := ret $ (abort (var 0 Ctx.Var.shead) A)
+
+theorem Eqv.zero_eq {A : Ty α} {Γ : Ctx α ε} {L : LCtx α}
+  (r s : Eqv φ (⟨Ty.empty, ⊥⟩::Γ) (A::L))
+  : r = s
+  := by apply Eqv.initial; exact ⟨(Ty.empty, ⊥), by simp, Ty.IsInitial.empty, rfl⟩
+
+theorem Eqv.zero_seq {A B : Ty α} {Γ : Ctx α ε} {L : LCtx α}
+  (r : Eqv φ (⟨A, ⊥⟩::Γ) (B::L))
+  : Eqv.zero ;; r = Eqv.zero
+  := zero_eq _ _
+
+def Eqv.lzero {Γ : Ctx α ε} {L : LCtx α} {A : Ty α}
+  : Eqv φ (⟨Ty.empty.coprod A, ⊥⟩::Γ) (A::L)
+  := coprod zero nil
+
+def Eqv.rzero {Γ : Ctx α ε} {L : LCtx α} {A : Ty α}
+  : Eqv φ (⟨A.coprod Ty.empty, ⊥⟩::Γ) (A::L)
+  := coprod nil zero
+
+def Eqv.inj_l {A B : Ty α} {Γ : Ctx α ε} {L : LCtx α}
+  : Eqv φ (⟨A, ⊥⟩::Γ) (A.coprod B::L)
+  := ret (inl (var 0 Ctx.Var.shead))
+
+def Eqv.inj_r {A B : Ty α} {Γ : Ctx α ε} {L : LCtx α}
+  : Eqv φ (⟨B, ⊥⟩::Γ) (A.coprod B::L)
+  := ret (inr (var 0 Ctx.Var.shead))
+
+theorem Eqv.Pure.lzero {Γ : Ctx α ε} {L : LCtx α} {A : Ty α}
+  : (lzero (φ := φ) (Γ := Γ) (L := L) (A := A)).Pure := sorry
+
+theorem Eqv.Pure.rzero {Γ : Ctx α ε} {L : LCtx α} {A : Ty α}
+  : (rzero (φ := φ) (Γ := Γ) (L := L) (A := A)).Pure := sorry
+
+theorem Eqv.Pure.inj_l {A B : Ty α} {Γ : Ctx α ε} {L : LCtx α}
+  : (inj_l (φ := φ) (Γ := Γ) (L := L) (A := A) (B := B)).Pure
+  := ⟨inl (var 0 Ctx.Var.shead), rfl⟩
+
+theorem Eqv.Pure.inj_r {A B : Ty α} {Γ : Ctx α ε} {L : LCtx α}
+  : (inj_r (φ := φ) (Γ := Γ) (L := L) (A := A) (B := B)).Pure
+  := ⟨inr (var 0 Ctx.Var.shead), rfl⟩
+
+def Eqv.sum {A B C D : Ty α} {Γ : Ctx α ε} {L : LCtx α}
+  (l : Eqv φ (⟨A, ⊥⟩::Γ) (C::L)) (r : Eqv φ (⟨B, ⊥⟩::Γ) (D::L))
+  : Eqv φ (⟨A.coprod B, ⊥⟩::Γ) ((C.coprod D)::L)
+  := coprod (l ;; inj_l) (r ;; inj_r)
+
+theorem Eqv.Pure.sum {A B C D : Ty α} {Γ : Ctx α ε} {L : LCtx α}
+  {l : Eqv φ (⟨A, ⊥⟩::Γ) (C::L)} (hl : l.Pure)
+  {r : Eqv φ (⟨B, ⊥⟩::Γ) (D::L)} (hr : r.Pure)
+  : (sum l r).Pure := coprod (seq hl inj_l) (seq hr inj_r)
+
+theorem Eqv.coprod_inl_inr {A B : Ty α} {Γ : Ctx α ε} {L : LCtx α}
+  : coprod inj_l inj_r = Eqv.nil (φ := φ) (ty := A.coprod B) (rest := Γ) (targets := L) := by
+  -- TODO: case_eta
+  sorry
+
+theorem Eqv.sum_nil {A B : Ty α} {Γ : Ctx α ε} {L : LCtx α}
+  : sum (φ := φ) (A := A) (B := B) (Γ := Γ) (L := L) nil nil = nil := coprod_inl_inr
+
+theorem Eqv.inj_l_coprod {A B C : Ty α} {Γ : Ctx α ε} {L : LCtx α}
+  (l : Eqv φ (⟨A, ⊥⟩::Γ) (C::L)) (r : Eqv φ (⟨B, ⊥⟩::Γ) (C::L))
+  : inj_l ;; coprod l r = l := by
+  stop
+  rw [inj_l, coprod, ret_seq, vwk1, vwk_case, vsubst_case]
+  simp only [Set.mem_setOf_eq, wk_var, Nat.liftWk_zero, subst_var, Term.Subst.InS.get_0_subst0]
+  rw [case_inl, let1_beta, vwk1, vwk_vwk, vsubst_vsubst]
+  -- TODO: vwk_vsubst, lore...
+  sorry
+
+theorem Eqv.inj_r_coprod {A B C : Ty α} {Γ : Ctx α ε} {L : LCtx α}
+  (l : Eqv φ (⟨A, ⊥⟩::Γ) (C::L)) (r : Eqv φ (⟨B, ⊥⟩::Γ) (C::L))
+  : inj_r ;; coprod l r = r := by
+  stop
+  rw [inj_r, coprod, ret_seq, vwk1, vwk_case, vsubst_case]
+  simp only [Set.mem_setOf_eq, wk_var, Nat.liftWk_zero, subst_var, Term.Subst.InS.get_0_subst0]
+  rw [case_inr, let1_beta, vwk1, vwk_vwk, vsubst_vsubst]
+  -- TODO: vwk_vsubst, lore...
+  sorry
+
+theorem Eqv.inj_l_rzero
+  : inj_l ;; rzero = nil (φ := φ) (ty := A) (rest := Γ) (targets := L) := by
+  rw [rzero, inj_l_coprod]
+
+theorem Eqv.inj_r_lzero
+  : inj_r ;; lzero = nil (φ := φ) (ty := A) (rest := Γ) (targets := L) := by
+  rw [lzero, inj_r_coprod]
+
+theorem Eqv.rzero_inj_l {A : Ty α}
+  : rzero ;; inj_l = nil (φ := φ) (ty := A.coprod Ty.empty) (rest := Γ) (targets := L) := by
+  rw [rzero, coprod_seq, <-sum_nil, sum]
+  congr 1
+  apply zero_eq
+
+theorem Eqv.lzero_inj_r {A : Ty α}
+  : lzero ;; inj_r = nil (φ := φ) (ty := Ty.empty.coprod A) (rest := Γ) (targets := L) := by
+  rw [lzero, coprod_seq, <-sum_nil, sum]
+  congr 1
+  apply zero_eq
+
+-- TODO: naturality
+
+theorem Eqv.inj_l_join {Γ : Ctx α ε} {L : LCtx α}
+  : inj_l ;; join (φ := φ) (A := A) (Γ := Γ) (L := L) = nil := by
+  rw [join, inj_l_coprod]
+
+theorem Eqv.inj_r_join {Γ : Ctx α ε} {L : LCtx α}
+  : inj_r ;; join (φ := φ) (A := A) (Γ := Γ) (L := L) = nil := by
+  rw [join, inj_r_coprod]
+
+-- TODO: sum_nil_zero_join, sum_zero_nil_join for comonoid structure
+
+-- TODO: universal comonoid compatibility, so join merges everything
+
+theorem Eqv.inj_l_seq_sum {A B C D : Ty α} {Γ : Ctx α ε} {L : LCtx α}
+  (l : Eqv φ (⟨A, ⊥⟩::Γ) (C::L)) (r : Eqv φ (⟨B, ⊥⟩::Γ) (D::L))
+  : inj_l ;; (sum l r) = l ;; inj_l := by rw [sum, inj_l_coprod]
+
+theorem Eqv.inj_r_seq_sum {A B C D : Ty α} {Γ : Ctx α ε} {L : LCtx α}
+  (l : Eqv φ (⟨A, ⊥⟩::Γ) (C::L)) (r : Eqv φ (⟨B, ⊥⟩::Γ) (D::L))
+  : inj_r ;; (sum l r) = r ;; inj_r := by rw [sum, inj_r_coprod]
+
+theorem Eqv.sum_seq_coprod {A B C D E : Ty α} {Γ : Ctx α ε} {L : LCtx α}
+  (l : Eqv φ (⟨A, ⊥⟩::Γ) (C::L)) (r : Eqv φ (⟨B, ⊥⟩::Γ) (D::L))
+  (s : Eqv φ (⟨C, ⊥⟩::Γ) (E::L)) (t : Eqv φ (⟨D, ⊥⟩::Γ) (E::L))
+  : (sum l r) ;; (coprod s t) = coprod (l ;; s) (r ;; t) := by
+  rw [sum, coprod_seq, seq_assoc, inj_l_coprod, seq_assoc, inj_r_coprod]
+
+theorem Eqv.sum_seq_sum {A B C D E F : Ty α} {Γ : Ctx α ε} {L : LCtx α}
+  (l : Eqv φ (⟨A, ⊥⟩::Γ) (C::L)) (r : Eqv φ (⟨B, ⊥⟩::Γ) (D::L))
+  (s : Eqv φ (⟨C, ⊥⟩::Γ) (E::L)) (t : Eqv φ (⟨D, ⊥⟩::Γ) (F::L))
+  : (sum l r) ;; (sum s t) = sum (l ;; s) (r ;; t) := by
+  rw [sum, coprod_seq, seq_assoc, inj_l_seq_sum, seq_assoc, inj_r_seq_sum]
+  simp only [<-seq_assoc]; rfl
+
+theorem Eqv.sum_seq_join {A B C : Ty α} {Γ : Ctx α ε} {L : LCtx α}
+  (l : Eqv φ (⟨A, ⊥⟩::Γ) (C::L)) (r : Eqv φ (⟨B, ⊥⟩::Γ) (C::L))
+  : (sum l r) ;; join = coprod l r := by simp [join, sum_seq_coprod]
+
+theorem Eqv.sum_self_seq_join {A B} {Γ : Ctx α ε} {L : LCtx α}
+  (r : Eqv φ (⟨A, ⊥⟩::Γ) (B::L))
+  : sum r r ;; join = join ;; r := by rw [sum_seq_join, join, coprod_seq]; simp
+
+def Eqv.braid_sum {A B : Ty α} {Γ : Ctx α ε} {L : LCtx α}
+  : Eqv φ (⟨A.coprod B, ⊥⟩::Γ) (B.coprod A::L)
+  := coprod inj_r inj_l
+
+theorem Eqv.Pure.braid_sum {A B : Ty α} {Γ : Ctx α ε} {L : LCtx α}
+  : (braid_sum (φ := φ) (A := A) (B := B) (Γ := Γ) (L := L)).Pure := coprod inj_r inj_l
+
+theorem Eqv.braid_sum_seq_braid_sum {A B : Ty α} {Γ : Ctx α ε} {L : LCtx α}
+  : braid_sum (φ := φ) (A := A) (B := B) (Γ := Γ) (L := L) ;; braid_sum = nil := by
+  simp only [braid_sum, coprod_seq, inj_l_coprod, inj_r_coprod, coprod_inl_inr]
+
+theorem Eqv.braid_sum_seq_coprod {A B C : Ty α} {Γ : Ctx α ε} {L : LCtx α}
+  (l : Eqv φ (⟨A, ⊥⟩::Γ) (C::L)) (r : Eqv φ (⟨B, ⊥⟩::Γ) (C::L))
+  : braid_sum ;; (coprod l r) = coprod r l := by
+  rw [braid_sum, coprod_seq, inj_l_coprod, inj_r_coprod]
+
+theorem Eqv.braid_sum_seq_sum {A B C D : Ty α} {Γ : Ctx α ε} {L : LCtx α}
+  (l : Eqv φ (⟨A, ⊥⟩::Γ) (C::L)) (r : Eqv φ (⟨B, ⊥⟩::Γ) (D::L))
+  : braid_sum ;; (sum l r) = sum r l ;; braid_sum := by
+  rw [sum, braid_sum_seq_coprod, braid_sum, sum_seq_coprod]
+
+def Eqv.assoc_sum {A B C : Ty α} {Γ : Ctx α ε} {L : LCtx α}
+  : Eqv φ (⟨(A.coprod B).coprod C, ⊥⟩::Γ) (A.coprod (B.coprod C)::L)
+  := sorry
+
+def Eqv.assoc_inv_sum {A B C : Ty α} {Γ : Ctx α ε} {L : LCtx α}
+  : Eqv φ (⟨A.coprod (B.coprod C), ⊥⟩::Γ) ((A.coprod B).coprod C::L)
+  := sorry
+
+theorem Eqv.Pure.assoc_sum {A B C : Ty α} {Γ : Ctx α ε} {L : LCtx α}
+  : (assoc_sum (φ := φ) (A := A) (B := B) (C := C) (Γ := Γ) (L := L)).Pure := sorry
+
+theorem Eqv.Pure.assoc_inv_sum {A B C : Ty α} {Γ : Ctx α ε} {L : LCtx α}
+  : (assoc_inv_sum (φ := φ) (A := A) (B := B) (C := C) (Γ := Γ) (L := L)).Pure := sorry
+
+theorem Eqv.assoc_assoc_inv_sum {A B C : Ty α} {Γ : Ctx α ε} {L : LCtx α}
+  : assoc_sum (φ := φ) (A := A) (B := B) (C := C) (Γ := Γ) (L := L) ;; assoc_inv_sum = nil
+  := sorry
+
+theorem Eqv.assoc_inv_assoc_sum {A B C : Ty α} {Γ : Ctx α ε} {L : LCtx α}
+  : assoc_inv_sum (φ := φ) (A := A) (B := B) (C := C) (Γ := Γ) (L := L) ;; assoc_sum = nil
+  := sorry
+
+theorem Eqv.assoc_sum_nat {A B C A' B' C' : Ty α} {Γ : Ctx α ε} {L : LCtx α}
+  (l : Eqv φ (⟨A, ⊥⟩::Γ) (A'::L)) (m : Eqv φ (⟨B, ⊥⟩::Γ) (B'::L)) (r : Eqv φ (⟨C, ⊥⟩::Γ) (C'::L))
+  : sum (sum l m) r ;; assoc_sum = assoc_sum ;; sum l (sum m r) := sorry
+
+theorem Eqv.triangle_sum {X Y : Ty α} {Γ : Ctx α ε} {L : LCtx α}
+  : assoc_sum (φ := φ) (Γ := Γ) (L := L) (A := X) (B := Ty.empty) (C := Y) ;; nil.sum lzero
+  = rzero.sum nil := sorry
+
+theorem Eqv.pentagon_sum {W X Y Z : Ty α} {Γ : Ctx α ε} {L : LCtx α}
+  : assoc_sum (φ := φ) (Γ := Γ) (L := L) (A := W.coprod X) (B := Y) (C := Z) ;; assoc_sum
+  = assoc_sum.sum nil ;; assoc_sum ;; nil.sum assoc_sum := sorry
+
+theorem Eqv.hexagon_sum {X Y Z : Ty α} {Γ : Ctx α ε} {L : LCtx α}
+  : assoc_sum (φ := φ) (Γ := Γ) (L := L) (A := X) (B := Y) (C := Z) ;; braid_sum ;; assoc_sum
+  = braid_sum.sum nil ;; assoc_sum ;; nil.sum braid_sum := sorry
